

Task 4

$$L(g, \eta) = g^T \nabla_0 J + \eta (\epsilon - g^T F g)$$

$$\frac{\partial L(g, \eta)}{\partial g} = \nabla_0 J - 2\eta F g \stackrel{!}{=} 0 \Leftrightarrow \nabla_0 J = 2\eta F g$$

$$g = (2\eta F)^{-1} \nabla_0 J = \frac{1}{2} \eta^{-1} F^{-1} \nabla_0 J$$

$$g(g^*, \eta) = \left(\frac{1}{2} \eta^{-1} F^{-1} \nabla_0 J \right)^T \nabla_0 J + \eta (\epsilon - \left(\frac{1}{2} \eta^{-1} F^{-1} \nabla_0 J \right)^T F \left(\frac{1}{2} \eta^{-1} F^{-1} \nabla_0 J \right))$$

$$= \frac{1}{2} \eta^{-1} \nabla_0 J^T F^{-1} \nabla_0 J + \eta \epsilon - \eta \cancel{\frac{1}{2} \eta^{-1} \nabla_0 J^T F^{-1}} \cancel{F} \cancel{\frac{1}{2} \eta^{-1} F^{-1} \nabla_0 J}$$

$$= \frac{1}{2} \eta^{-1} \nabla_0 J^T F^{-1} \nabla_0 J + \eta \epsilon$$

$$\frac{\partial g(g^*, \eta)}{\partial \eta} = -\frac{1}{2} \eta^{-2} \nabla_0 J^T F^{-1} \nabla_0 J + \epsilon \stackrel{!}{=} 0$$

$$\rightarrow \eta^* = \sqrt{\frac{\epsilon}{\nabla_0 J^T F^{-1} \nabla_0 J}}$$